src/PlutusIR/Semantics/Dynamic/Bigstep/EvalValue.v
@@ -17,7 +17,16 @@ Proof with (autounfold; (eauto || (try lia))).
       eapply E_Constr_cons with (k_t := 0) (k_ts := 0)...
 Qed.
 
+Lemma eval_result' :
+  forall v, result' v -> v =[0]=> v.
+Admitted.
+
 Corollary eval_result__result : forall v,
     result v ->
     v =[0]=> v.
 Proof. apply eval_result. Qed.
+
+Corollary eval_result'__result' : forall v,
+    result' v ->
+    v =[0]=> v.
+Admitted.
