src/PlutusIR/Semantics/SemanticEquivalence/LogicalRelation/RG/Helpers.v
@@ -27,9 +27,9 @@ Proof.
 Qed.
 
 
-Lemma R_G_extend_rho : forall X Chi T1 T2 rho k c env env' ,
-    R_G rho k c env env' ->
-    R_G ((X, (Chi, T1, T2)) :: rho) k c env env'.
+Lemma G_extend_rho : forall X Chi T1 T2 rho k c env env' ,
+    G rho k c env env' ->
+    G ((X, (Chi, T1, T2)) :: rho) k c env env'.
 (* See comment in R_V_extend_rho, X may not occur in rho *)
 Admitted.
 
@@ -52,8 +52,8 @@ Proof.
       assumption.
 Qed.
 
-Lemma R_G_domains_match : forall c e1 e2 k rho,
-    R_G rho k c e1 e2 ->
+Lemma G_domains_match : forall c e1 e2 k rho,
+    G rho k c e1 e2 ->
     forall x T,
       lookup x c = Datatypes.Some T ->
       exists v1 v2,
@@ -77,8 +77,8 @@ Proof.
     + eauto.
 Qed.
 
-Lemma R_G_context_normal : forall rho k c e1 e2,
-    R_G rho k c e1 e2 ->
+Lemma G_context_normal : forall rho k c e1 e2,
+    G rho k c e1 e2 ->
     forall x T,
       lookup x c = Datatypes.Some T ->
       normal_Ty T.
@@ -110,8 +110,8 @@ Proof.
 Qed.
 
 
-Lemma R_G_env_closed : forall rho k c e1 e2,
-    R_G rho k c e1 e2 ->
+Lemma G_env_closed : forall rho k c e1 e2,
+    G rho k c e1 e2 ->
     closed_env e1 /\ closed_env e2.
 Admitted.
 
@@ -122,10 +122,10 @@ Corollary RG_env_closed_1 : forall rho k c e1 e2,
 Proof. intros. destruct (RG_env_closed _ _ _ _ _ H H0). assumption. Qed.
 
 
-Corollary R_G_env_closed_1 : forall rho k c e1 e2,
-    R_G rho k c e1 e2 ->
+Corollary G_env_closed_1 : forall rho k c e1 e2,
+    G rho k c e1 e2 ->
     closed_env e1.
-Proof. intros. destruct (R_G_env_closed _ _ _ _ _ H). assumption. Qed.
+Proof. intros. destruct (G_env_closed _ _ _ _ _ H). assumption. Qed.
 
 Corollary RG_env_closed_2 : forall rho k c e1 e2,
     RG rho k c e1 e2 ->
@@ -134,10 +134,10 @@ Corollary RG_env_closed_2 : forall rho k c e1 e2,
 Proof. intros. destruct (RG_env_closed _ _ _ _ _ H H0). assumption. Qed.
 
 
-Corollary R_G_env_closed_2 : forall rho k c e1 e2,
-    R_G rho k c e1 e2 ->
+Corollary G_env_closed_2 : forall rho k c e1 e2,
+    G rho k c e1 e2 ->
     closed_env e2.
-Proof. intros. destruct (R_G_env_closed _ _ _ _ _ H). assumption. Qed.
+Proof. intros. destruct (G_env_closed _ _ _ _ _ H). assumption. Qed.
 
 Lemma RG_RV : forall rho k c e1 e2,
     RG rho k c e1 e2 ->
@@ -159,13 +159,13 @@ Proof.
     + apply IHV with x'; assumption.
 Qed.
 
-Lemma R_G_R_V : forall rho k c e1 e2,
-    R_G rho k c e1 e2 ->
+Lemma G__V : forall rho k c e1 e2,
+    G rho k c e1 e2 ->
     forall x T v1 v2,
       lookup x c = Datatypes.Some T ->
       lookup x e1 = Datatypes.Some v1 ->
       lookup x e2 = Datatypes.Some v2 ->
-      R_V k T rho v1 v2.
+      V k T rho v1 v2.
 Admitted.
 
 Lemma RG_drop : forall rho k c e1 e2,
@@ -186,10 +186,10 @@ Proof.
       * apply IHV.
 Qed.
 
-Lemma R_G_drop : forall rho k c e1 e2,
-    R_G rho k c e1 e2 ->
+Lemma G_drop : forall rho k c e1 e2,
+    G rho k c e1 e2 ->
     forall x,
-      R_G rho k (drop x c) (drop x e1) (drop x e2).
+      G rho k (drop x c) (drop x e1) (drop x e2).
 Admitted.
 
 Lemma RG_mdrop : forall xs rho k c e1 e2,
@@ -202,7 +202,7 @@ Proof with auto.
 Qed.
 
 
-Lemma R_G_mdrop : forall xs rho k c e1 e2,
-    R_G rho k c e1 e2 ->
-      R_G rho k (mdrop xs c) (mdrop xs e1) (mdrop xs e2).
+Lemma G_mdrop : forall xs rho k c e1 e2,
+    G rho k c e1 e2 ->
+      G rho k (mdrop xs c) (mdrop xs e1) (mdrop xs e2).
 Admitted.
